ulib/prims.fst
@@ -16,6 +16,7 @@
 module Prims
 
 assume new type hasEq: Type -> GTot Type0
+type eqtype = a:Type{hasEq a}
 
 (* False is the empty inductive type *)
 type c_False =
@@ -24,6 +25,10 @@ type c_False =
 type c_True =
   | T
 
+(*
+ * These definitions are just so that we can generate their interpretations for now
+ * Fix encoding by generating interpretations for inductives so that these can be removed
+ *)
 type l_True = c_True
 
 type l_False = c_False
@@ -86,9 +91,6 @@ type squash (p:Type) = x:unit{p}
   
 (* forall (x:a). p x : specialized to Type#0 *)
 type l_Forall (#a:Type) (p:a -> GTot Type0) = squash (x:a -> GTot (p x))
-
-(* eq2 is reflexive *)
-assume Eq2_refl: forall (a:Type) (b:Type) (x:a) (y:b). eq2 #a #b x y == eq2 #b #a y x
 
 (* dependent pairs DTuple2 in concrete syntax is '(x:a & b x)' *)
 type dtuple2 (a:Type)
