ulib/FStar.Int16.fst
@@ -11,6 +11,11 @@ let within_int16 (i:int) =
     min_value_int <= i
     && i <= max_value_int
 
+(*
+ * TODO: this is a hack, we should handle refinement types more uniformly
+ *)
+assume HasEq_within_int: hasEq (i:int{within_int16 i})
+
 private type int16 =
   | Int16 : i:int{within_int16 i} -> int16
 
