ulib/FStar.Int64.fst
@@ -10,6 +10,11 @@ let within_int64 (i:int) =
     min_value_int <= i
     && i <= max_value_int
 
+(*
+ * TODO: this is a hack, we should handle refinement types more uniformly
+ *)
+assume HasEq_within_int: hasEq (i:int{within_int64 i})
+
 private type int64 =
   | Int64 : i:int{within_int64 i} -> int64
 
